%\renewcommand{\theequation}{\theenumi}
\begin{enumerate}[label=\thesection.\arabic*.,ref=\thesection.\theenumi]
%\numberwithin{equation}{enumi}

%
\item From equation $\left(3.0.3\right)$... 
%
\begin{align}
\frac{1}{2}\norm{\vec{B}-\vec{C}} &= \frac{1}{2}\norm{\vec{Q}-\vec{R}}
 \\
 \norm{\vec{B}-\vec{M}} &= \norm{\vec{Q}-\vec{N}}
\end{align}

\item From fig $\left[2.1\right]$ ...

\begin{align}
\norm{\vec{A}-\vec{B}} &= \norm{\vec{P}-\vec{Q}} 
\\ 
\norm{\vec{A}-\vec{M}} &= \norm{\vec{P}-\vec{N}}
\\
\norm{\vec{B}-\vec{M}} &= \norm{\vec{Q}-\vec{N}}
\end{align}

$\implies$ from SSS congurance rule $\Delta ABM \cong \Delta PQN$
\end{enumerate}
