%\renewcommand{\theequation}{\theenumi}
\begin{enumerate}[label=\thesection.\arabic*.,ref=\thesection.\theenumi]
%\numberwithin{equation}{enumi}
	
\item
given that $\to$\\
\begin{align}
\norm{\vec{A}-\vec{M}} &= \norm{\vec{P}-\vec{N}} = m = n
\end{align}

from equation $\left(3.0.3\right)$...
\begin{align}
\frac{1}{2}\norm{\vec{B}-\vec{C}} &= \frac{1}{2}\norm{\vec{Q}-\vec{R}} 
 \\
 \norm{\vec{M}-\vec{C}} &= \norm{\vec{N}-\vec{R}} 
\end{align}

\begin{align}
\because \Delta ABM \cong \Delta PQN 
\\
\implies \angle AMB = \angle PNQ
\\
180 - \angle AMB = 180 -  \angle PNQ
\\
\angle AMC = \angle PNR
\end{align}


from equation $\left(3.0.2\right)$,$\left(3.2.3\right)$ and $\left(3.2.10\right)$...
\begin{align}
\norm{\vec{A}-\vec{M}} &= \norm{\vec{P}-\vec{N}}
\\
\norm{\vec{M}-\vec{C}} &= \norm{\vec{N}-\vec{R}}
\\
\angle AMC = \angle PNR
\end{align}
$\implies$ from SAS congurancy $ \Delta AMC \cong \Delta PNR$
\\
%
$\implies \norm{\vec{A}-\vec{C}} =\norm{\vec{P}-\vec{R}}$

	from equation $\left(3.0.1\right)$,$\left(3.0.3\right)$ and...
\begin{align}
\norm{\vec{A}-\vec{B}} &= \norm{\vec{P}-\vec{Q}}
\\
\norm{\vec{B}-\vec{C}} &= \norm{\vec{Q}-\vec{R}}
\\
\norm{\vec{A}-\vec{C}} &= \norm{\vec{P}-\vec{R}}
\end{align}

$\implies$ from SSS congurancy $\Delta ABC \cong \Delta PQR$



\end{enumerate}
